providers/quic/Spec.QUIC.fst
@@ -1486,7 +1486,7 @@ let rec xor_inplace_commutative (b b1 b2:bytes) (pos1 pos2:nat) : Lemma
   FStar.Classical.forall_intro step
 
 
-let rec and_inplace (b1 b2:bytes) (pos:nat)
+let and_inplace (b1 b2:bytes) (pos:nat)
   : Pure bytes
   (requires S.length b2 + pos <= S.length b1)
   (ensures fun b -> S.length b == S.length b1)
@@ -1506,7 +1506,7 @@ packet[pn_offset..pn_offset+4] ^= pn_mask &
   | 2 -> mask & 0xFFFFFF00
   | 3 -> mask & 0xFFFFFFFF
 *)
-inline_for_extraction private
+inline_for_extraction
 let pn_sizemask (pn_len:nat2) : lbytes 4 =
   let open FStar.Endianness in
   n_to_be 4 (pow2 32 - pow2 (24 - (8 `op_Multiply` pn_len)))
@@ -1527,15 +1527,19 @@ let block_of_sample a (k: Cipher.key a) (sample: lbytes 16): lbytes 16 =
   in
   S.slice (Cipher.ctr_block a k iv ctr) 0 16
 
+let pn_offset h =
+  assert_norm(max_cipher_length < pow2 62);
+  match h with
+    | Short _ _ cid -> 1 + S.length cid
+    | Long _ _ dcil scil _ _ pl -> 6 + add3 dcil + add3 scil + vlen pl
+
 let header_encrypt a hpk h npn c =
   assert_norm(max_cipher_length < pow2 62);
-  let pn_offset = match h with
-    | Short _ _ cid -> 1 + S.length cid
-    | Long _ _ dcil scil _ _ pl -> 6 + add3 dcil + add3 scil + vlen pl in
+  let pn_offset = pn_offset h in
   let pn_len = S.length npn - 1 in
   let sample = S.slice c (3-pn_len) (19-pn_len) in
   let mask = block_of_sample (AEAD.cipher_alg_of_supported_alg a) hpk sample in
-  let pnmask = and_inplace (S.slice mask 1 5) (pn_sizemask pn_len) 0 in
+  let pnmask = and_inplace (pn_sizemask pn_len) (S.slice mask 1 5) 0 in
   let sflags = if Short? h then 0x1fuy else 0x0fuy in
   let fmask = S.create 1 U8.(S.index mask 0 `logand` sflags) in
   let r = S.(format_header h npn @| c) in
@@ -2590,6 +2594,7 @@ let encrypt a k siv hpk pn_len seqn h plain =
   assert_norm(pow2 62 < pow2 (8 `op_Multiply` 12));
   // packet number bytes
   let pnb = FStar.Endianness.n_to_be 12 seqn in
+  // network packet number: truncated lower bytes
   let npn : lbytes (1+pn_len) = S.slice pnb (11 - pn_len) 12 in
   let header = format_header h npn in
   lemma_format_len a h npn;
